Progress with clos_remove correctness
Prove first of two important subsidiary lemmas: that if removal is done
over a list of possibly unnecessary environment values, then evaluating
this list starting in related states, results in suitably related value
lists, and related states. Here "suitably related" means that values are
related if they weren't dropped.

Second lemma is to show that evaluating in suitably related environments
where things have been dropped only in accordance with free variables
being present or not results in related results.

compiler/backend/proofs/clos_removeProofScript.sml
@@ -296,9 +296,31 @@ val pure_expressions_clean = save_thm(
   pure_expressions_clean0 |> Q.SPECL [`[e]`, `env`, `s`]
                           |> SIMP_RULE (srw_ss()) [])
 
-(*
+val keepval_rel_def = Define`
+  keepval_rel tyit c kis i v1 v2 =
+    if i ∈ kis then val_rel tyit c v1 v2
+    else v2 = Number 0
+`;
+
+val keepval_rel_o_SUC = Q.store_thm(
+  "keepval_rel_o_SUC",
+  `keepval_rel tyit c kis o SUC =
+      keepval_rel tyit c (kis o SUC)`,
+  simp[keepval_rel_def, FUN_EQ_THM, SPECIFICATION]);
+
+val GSPEC_o = Q.store_thm(
+  "GSPEC_o",
+  `GSPEC f o g = { x | ∃y. (g x, T) = f y }`,
+  simp[FUN_EQ_THM, GSPECIFICATION]);
+
+val ELplus1 = Q.store_thm(
+  "ELplus1",
+  `EL (n + 1) l = EL n (TL l)`,
+  simp[GSYM ADD1, EL]);
+
 val evaluate_MAPrm1 = Q.prove(
-  `(∀e es' vs. MEM e es ∧ remove [e] = (es', vs) ⇒ exp_rel (:'ffi) [e] es') ∧
+  `(∀e i es' vs. MEM e es ∧ mustkeep i e keeps ∧ remove [e] = (es', vs) ⇒
+                 exp_rel (:'ffi) [e] es') ∧
    LIST_REL (val_rel (:'ffi) i) env1 env2 ∧
    state_rel i (s1:'ffi closSem$state) s2 ∧ j ≤ i ⇒
      case evaluate (es, env1, s1 with clock := j) of
@@ -307,9 +329,8 @@ val evaluate_MAPrm1 = Q.prove(
             evaluate (MAPi (rm1 keeps b) es, env2, s2 with clock := j) =
               (Rval vs', s') ∧
             state_rel s.clock s s' ∧
-            LIST_RELi (λi v1 v2. if mustkeep (b + i) (EL i es) keeps then
-                                   val_rel (:'ffi) s.clock v1 v2
-                                 else v2 = Number 0)
+            LIST_RELi (keepval_rel (:'ffi) s.clock
+                         { i | mustkeep (b + i) (EL i es) keeps })
                       vs
                       vs'
      | (Rerr e, s) =>
@@ -338,7 +359,7 @@ val evaluate_MAPrm1 = Q.prove(
           simp[] >> qcase_tac `remove [e]` >> Cases_on `remove [e]` >>
           imp_res_tac remove_SING >> var_eq_tac >> fs[] >>
           qcase_tac `remove [e] = ([e'], _)` >>
-          qpat_assum `exp_rel _ _ _` mp_tac >>
+          first_x_assum (qspec_then `b` mp_tac) >> simp[] >>
           simp[exp_rel_def, exec_rel_rw, evaluate_ev_def] >>
           disch_then (qspecl_then [`i`, `env1`, `env2`, `s1`, `s2`] mp_tac) >>
           simp[] >> disch_then (qspec_then `j` mp_tac) >> simp[res_rel_rw] >>
@@ -348,9 +369,112 @@ val evaluate_MAPrm1 = Q.prove(
       simp[rm1_def] >>
       asm_simp_tac (srw_ss() ++ COND_elim_ss ++ CONJ_ss)
         [closSemTheory.evaluate_def, const_0_def, closSemTheory.do_app_def] >>
-      reverse (Cases
-*)
-
+      reverse (Cases_on `mustkeep b e keeps`) >> simp[]
+      >- (fs[mustkeep_def] >>
+          IMP_RES_THEN (qspecl_then [`s1 with clock := j`, `env1`] mp_tac)
+                       pure_expressions_clean >> simp[]) >>
+      qcase_tac `remove [e]` >> Cases_on `remove [e]` >>
+      imp_res_tac remove_SING >> var_eq_tac >> fs[] >>
+      first_x_assum (qspec_then `b` mp_tac) >> simp[] >>
+      simp[exp_rel_def, exec_rel_rw, evaluate_ev_def] >>
+      disch_then (qspecl_then [`i`, `env1`, `env2`, `s1`, `s2`] mp_tac) >>
+      simp[] >> disch_then (qspec_then `j` mp_tac) >> simp[res_rel_rw]) >>
+  qcase_tac `evaluate _ = (Rval r1list, s1')` >>
+  `∃r1. r1list = [r1]` by metis_tac[evaluate_SING] >> var_eq_tac >> simp[] >>
+  `∃r1' s1''. evaluate (es,env1,s1') = (r1',s1'')`
+     by metis_tac[pair_CASES] >> simp[] >>
+  reverse (Cases_on `r1'`) >> simp[]
+  >- (qcase_tac `evaluate(es,env1,s1') = (Rerr err, s1'')` >>
+      Cases_on `err` >> simp[res_rel_rw]
+      >- (simp[rm1_def] >> reverse (Cases_on `mustkeep b e keeps`) >> simp[]
+          >- (dsimp[const_0_def, closSemTheory.evaluate_def,
+                    closSemTheory.do_app_def, rm1_o_SUC, pair_case_eq, eqs] >>
+              fs[mustkeep_def] >>
+              IMP_RES_THEN (qspecl_then [`s1 with clock := j`, `env1`] mp_tac)
+                           pure_expressions_clean >> simp[] >> rw[] >>
+              first_x_assum
+                (qspecl_then [`s1`, `s2`, `j`, `i`, `b + 1`, `env1`, `env2`]
+                             mp_tac) >>
+              simp[res_rel_rw] >> asm_rewrite_tac[]) >>
+          Cases_on `remove[e]` >> imp_res_tac remove_SING >> var_eq_tac >>
+          fs[] >> first_x_assum (qspec_then `b` mp_tac) >> simp[] >>
+          simp[exp_rel_def, exec_rel_rw, evaluate_ev_def] >>
+          disch_then (qspecl_then [`i`, `env1`, `env2`, `s1`, `s2`] mp_tac) >>
+          simp[] >> disch_then (qspec_then `j` mp_tac) >>
+          dsimp[res_rel_rw, rm1_o_SUC] >> rpt strip_tac >>
+          qcase_tac `state_rel s1'.clock s1' s2'` >>
+          first_x_assum (qspecl_then [`s1'`, `s2'`, `s2'.clock`, `s2'.clock`,
+                                      `b + 1`, `env1`, `env2`] mp_tac) >>
+          fs[] >> asm_rewrite_tac[] >>
+          `s1' with clock := s2'.clock = s1' ∧
+           s2' with clock := s2'.clock = s2'`
+            by simp[closSemTheory.state_component_equality] >>
+          dsimp[res_rel_rw, eqs, pair_case_eq] >> disch_then irule >>
+          irule val_rel_mono_list >> qexists_tac `i` >> simp[] >>
+          imp_res_tac closSemTheory.evaluate_clock >> fs[] >> simp[]) >>
+      qcase_tac `evaluate (es,_,_) = (Rerr (Rabort abt), _)` >>
+      Cases_on `abt` >> simp[res_rel_rw] >>
+      simp[rm1_def] >> reverse (Cases_on `mustkeep b e keeps`) >> simp[]
+      >- (dsimp[const_0_def, closSemTheory.evaluate_def,
+                closSemTheory.do_app_def, rm1_o_SUC, pair_case_eq, eqs] >>
+          fs[mustkeep_def] >>
+          IMP_RES_THEN (qspecl_then [`s1 with clock := j`, `env1`] mp_tac)
+                       pure_expressions_clean >> simp[] >> rw[] >>
+          first_x_assum
+            (qspecl_then [`s1`, `s2`, `j`, `i`, `b + 1`, `env1`, `env2`]
+                         mp_tac) >>
+          simp[res_rel_rw] >> asm_rewrite_tac[]) >>
+      Cases_on `remove[e]` >> imp_res_tac remove_SING >> var_eq_tac >>
+      fs[] >> first_x_assum (qspec_then `b` mp_tac) >> simp[] >>
+      simp[exp_rel_def, exec_rel_rw, evaluate_ev_def] >>
+      disch_then (qspecl_then [`i`, `env1`, `env2`, `s1`, `s2`] mp_tac) >>
+      simp[] >> disch_then (qspec_then `j` mp_tac) >>
+      dsimp[res_rel_rw, rm1_o_SUC] >> rpt strip_tac >>
+      qcase_tac `state_rel s1'.clock s1' s2'` >>
+      first_x_assum (qspecl_then [`s1'`, `s2'`, `s2'.clock`, `s2'.clock`,
+                                  `b + 1`, `env1`, `env2`] mp_tac) >>
+      fs[] >> asm_rewrite_tac[] >>
+      `s1' with clock := s2'.clock = s1' ∧
+       s2' with clock := s2'.clock = s2'`
+        by simp[closSemTheory.state_component_equality] >>
+      dsimp[res_rel_rw, eqs, pair_case_eq] >> disch_then irule >>
+      irule val_rel_mono_list >> qexists_tac `i` >> simp[] >>
+      imp_res_tac closSemTheory.evaluate_clock >> fs[] >> simp[]) >>
+  simp[rm1_def] >> reverse (Cases_on `mustkeep b e keeps`) >> simp[]
+  >- (dsimp[const_0_def, closSemTheory.evaluate_def,
+            closSemTheory.do_app_def, rm1_o_SUC, pair_case_eq, eqs] >>
+      fs[mustkeep_def] >>
+      IMP_RES_THEN (qspecl_then [`s1 with clock := j`, `env1`] mp_tac)
+                   pure_expressions_clean >> simp[] >> rw[] >>
+      first_x_assum
+        (qspecl_then [`s1`, `s2`, `j`, `i`, `b + 1`, `env1`, `env2`]
+                     mp_tac) >>
+      simp[res_rel_rw] >>
+      simp[LIST_RELi_thm, combinTheory.o_ABS_L, ADD1, keepval_rel_def,
+           keepval_rel_o_SUC, GSPEC_o, ELplus1] >>
+      metis_tac[]) >>
+  Cases_on `remove[e]` >> imp_res_tac remove_SING >> var_eq_tac >>
+  fs[] >> first_x_assum (qspec_then`b` mp_tac) >> simp[] >>
+  simp[exp_rel_def, exec_rel_rw, evaluate_ev_def] >>
+  disch_then (qspecl_then [`i`, `env1`, `env2`, `s1`, `s2`] mp_tac) >>
+  simp[] >> disch_then (qspec_then `j` mp_tac) >>
+  dsimp[res_rel_rw, rm1_o_SUC] >> rpt strip_tac >>
+  dsimp[LIST_RELi_thm, combinTheory.o_ABS_L, ADD1, eqs, pair_case_eq,
+        keepval_rel_o_SUC, GSPEC_o, ELplus1, keepval_rel_def] >>
+  qcase_tac `state_rel s1'.clock s1' s2'` >>
+  first_x_assum (qspecl_then [`s1'`, `s2'`, `s2'.clock`, `s2'.clock`,
+                              `b + 1`, `env1`, `env2`] mp_tac) >>
+  fs[] >> asm_rewrite_tac[] >>
+  `s1' with clock := s2'.clock = s1' ∧
+   s2' with clock := s2'.clock = s2'`
+    by simp[closSemTheory.state_component_equality] >>
+  dsimp[res_rel_rw, eqs, pair_case_eq] >>
+  `LIST_REL (val_rel (:'ffi) s2'.clock) env1 env2`
+     by (irule val_rel_mono_list >> qexists_tac `i` >> simp[] >>
+         imp_res_tac closSemTheory.evaluate_clock >> lfs[]) >>
+  dsimp[] >> rpt strip_tac >> irule (hd (CONJUNCTS val_rel_mono)) >>
+  qexists_tac `s2'.clock` >> simp[] >>
+  imp_res_tac closSemTheory.evaluate_clock >> lfs[])
 
 val remove_correct = Q.store_thm("remove_correct",
   `∀es es' s.
@@ -370,7 +494,25 @@ val remove_correct = Q.store_thm("remove_correct",
        qx_genl_tac [`i`, `env1`, `env2`, `s1`, `s2`] >>
        strip_tac >>
        asm_simp_tac (srw_ss() ++ ETA_ss)
-         [closSemTheory.evaluate_def,GSYM rm1_def] >> cheat) >>
+         [closSemTheory.evaluate_def, GSYM mustkeep_def,
+          rm1_def |> GSYM |> SPEC_ALL
+                  |> Q.INST [`n` |-> `0`] |> SIMP_RULE (srw_ss()) []] >>
+       qx_gen_tac `j` >> strip_tac >>
+       qcase_tac `remove [body] = ([body'], keeps)` >>
+       qcase_tac `MEM _ es` >> mp_tac (Q.INST [`b` |-> `0`] evaluate_MAPrm1) >>
+       simp[] >> fs[GSYM mustkeep_def] >>
+       `∀e. MEM e es ⇒ every_Fn_vs_NONE [e]`
+          by fs[Once every_Fn_vs_NONE_EVERY, EVERY_MEM] >> fs[] >>
+       fs[PULL_FORALL, AND_IMP_INTRO, GSYM CONJ_ASSOC] >> asm_rewrite_tac[] >>
+       `∃r1 s1'. evaluate (es,env1,s1 with clock := j) = (r1,s1')`
+          by metis_tac[pair_CASES] >> simp[] >>
+       reverse (Cases_on `r1`) >> simp[]
+       >- (qcase_tac `evaluate _ = (Rerr err, s1')` >>
+           Cases_on `err` >> dsimp[res_rel_rw] >- metis_tac[] >>
+           qcase_tac `evaluate _ = (Rerr (Rabort abt), s1')` >>
+           Cases_on `abt` >> dsimp[res_rel_rw]) >>
+       dsimp[] >>
+       cheat) >>
   TRY (qcase_tac`Letrec` >>
        lfs[FOLDR_UNZIP, FPAIR, PAIR_MAP, FST_UNZIP_MAPi, SND_UNZIP_MAPi,
            combinTheory.o_ABS_R, pairTheory.o_UNCURRY_R
